src/cose/verifiedinterop/Sign.fst
@@ -88,23 +88,7 @@ let mk_sig_structure_spec
     : GTot spect_evercddl_Sig_structure_pretty =
   Mkspect_evercddl_Sig_structure_pretty0 signature1 phdr (Inr (aad, payload))
 
-fn mk_sig_structure phdr aad payload #vphdr #vaad #vpayload
-  requires rel_evercddl_empty_or_serialized_map phdr vphdr
-  requires rel_evercddl_bstr aad vaad
-  requires rel_evercddl_bstr payload vpayload
-  returns r: _
-  ensures rel_evercddl_Sig_structure r (mk_sig_structure_spec vphdr vaad vpayload)
-  ensures pure (r.context == signature1)
-  ensures pure (r.body_protected == phdr)
-  ensures pure (r._x0 == Inr (aad, payload))
-{
-  rewrite emp as rel_either rel_unit rel_unit signature1 signature1;
-  rw_l (rel_sig_structure_eq (Mkevercddl_Sig_structure_pretty0 signature1 phdr (Inr (aad, payload)))
-    (Mkspect_evercddl_Sig_structure_pretty0 signature1 vphdr (Inr (vaad, vpayload))));
-  with res vres. assert rel_evercddl_Sig_structure res vres;
-  rewrite each vres as mk_sig_structure_spec vphdr vaad vpayload;
-  res
-}
+open Pulse.Lib.Trade
 
 ghost fn norm_r p s
   requires p
@@ -117,20 +101,35 @@ ghost fn norm_r p s
 let unfold_plus p lids =
   norm_r p [delta_only lids; iota; primops]
 
-ghost fn free_mk_sig_structure
-    (ss: evercddl_Sig_structure_pretty { ss.context == signature1 })
-    (phdr: _ { ss.body_protected == phdr })
-    aad (payload: _ { ss._x0 == Inr (aad, payload) })
-    #vphdr #vaad #vpayload
-  requires rel_evercddl_Sig_structure ss (mk_sig_structure_spec vphdr vaad vpayload)
-  ensures rel_evercddl_empty_or_serialized_map phdr vphdr
-  ensures rel_evercddl_bstr aad vaad
-  ensures rel_evercddl_bstr payload vpayload
+fn mk_sig_structure phdr aad payload
+  (#vphdr: erased _)
+  (#vaad: erased _)
+  (#vpayload: erased _)
+  requires rel_evercddl_empty_or_serialized_map phdr vphdr
+  requires rel_evercddl_bstr aad vaad
+  requires rel_evercddl_bstr payload vpayload
+  returns r: evercddl_Sig_structure_pretty
+  ensures rel_evercddl_Sig_structure r (mk_sig_structure_spec vphdr vaad vpayload)
+  ensures trade (rel_evercddl_Sig_structure r (mk_sig_structure_spec vphdr vaad vpayload))
+    (rel_evercddl_empty_or_serialized_map phdr vphdr ** rel_evercddl_bstr aad vaad ** rel_evercddl_bstr payload vpayload)
 {
-  rewrite each ss as (Mkevercddl_Sig_structure_pretty0 signature1 phdr (Inr (aad, payload)));
-  unfold_plus (rel_evercddl_Sig_structure _ _) [`%mk_sig_structure_spec];
-  rw_r (rel_sig_structure_eq _ _);
-  rewrite rel_either rel_unit rel_unit signature1 signature1 as emp;
+  rewrite emp as rel_either rel_unit rel_unit signature1 signature1;
+  rw_l (rel_sig_structure_eq (Mkevercddl_Sig_structure_pretty0 signature1 phdr (Inr (aad, payload)))
+    (Mkspect_evercddl_Sig_structure_pretty0 signature1 vphdr (Inr (reveal vaad, reveal vpayload))));
+  with res vres. assert rel_evercddl_Sig_structure res vres;
+  rewrite each vres as mk_sig_structure_spec vphdr vaad vpayload;
+
+  ghost fn aux ()
+    requires emp ** rel_evercddl_Sig_structure res (mk_sig_structure_spec vphdr vaad vpayload)
+    ensures rel_evercddl_empty_or_serialized_map phdr vphdr ** rel_evercddl_bstr aad vaad ** rel_evercddl_bstr payload vpayload
+  {
+    unfold_plus (rel_evercddl_Sig_structure _ _) [`%mk_sig_structure_spec];
+    rw_r (rel_sig_structure_eq _ _);
+    rewrite rel_either rel_unit rel_unit signature1 signature1 as emp;
+  };
+  intro_trade _ _ _ aux;
+
+  res
 }
 
 open EverCrypt.Ed25519
@@ -155,7 +154,8 @@ let sz_to_u32_safe (i: SizeT.t { SizeT.v i < pow2 32 }) : j:UInt32.t { UInt32.v 
 assume val abort () : stt unit emp (fun _ -> pure False)
 
 fn create_sig privkey phdr aad payload (sigbuf: AP.ptr UInt8.t)
-    #vphdr #vaad #vpayload #pprivkey (#vprivkey: erased (Seq.seq UInt8.t) { Seq.length vprivkey == 32 })
+    (#vphdr: erased _) (#vaad: erased _) (#vpayload: erased _) (#pprivkey: erased _)
+    (#vprivkey: erased (Seq.seq UInt8.t) { Seq.length vprivkey == 32 })
   requires AP.pts_to privkey #pprivkey vprivkey
   requires rel_evercddl_empty_or_serialized_map phdr vphdr
   requires rel_evercddl_bstr aad vaad
@@ -183,7 +183,7 @@ fn create_sig privkey phdr aad payload (sigbuf: AP.ptr UInt8.t)
   assert pure (SizeT.v written <= SizeT.v sz);
   assert pure (SizeT.v written <= 1024);
   assert_norm (1024 < pow2 32);
-  free_mk_sig_structure sig_struct phdr aad payload;
+  elim_trade _ _;
   if (written = 0sz) {
     abort ();
     with vsigbuf. rewrite AP.pts_to sigbuf vsigbuf as AP.pts_to sigbuf (spec_ed25519_sign vprivkey vsigbuf);
@@ -200,6 +200,325 @@ fn create_sig privkey phdr aad payload (sigbuf: AP.ptr UInt8.t)
     Vec.to_vec_pts_to arr;
     Vec.free arr;
   }
+}
+
+let rel_inl_map =
+  (CDDL.Pulse.Types.rel_slice_of_table (CDDL.Pulse.Bundle.Base.mk_eq_test_bij
+                    COSE.Format.spect_aux_env25_type_2_pretty_right
+                    COSE.Format.spect_aux_env25_type_2_pretty_left
+                    COSE.Format.spect_aux_env25_type_2_pretty_left_right
+                    COSE.Format.spect_aux_env25_type_2_pretty_right_left
+                    (CDDL.Pulse.Bundle.Base.mk_eq_test_bij COSE.Format.spect_evercddl_label_pretty_right
+                        COSE.Format.spect_evercddl_label_pretty_left
+                        COSE.Format.spect_evercddl_label_pretty_left_right
+                        COSE.Format.spect_evercddl_label_pretty_right_left
+                        (CDDL.Spec.EqTest.either_eq (CDDL.Pulse.Bundle.Base.mk_eq_test_bij COSE.Format.spect_evercddl_int_pretty_right
+                                COSE.Format.spect_evercddl_int_pretty_left
+                                COSE.Format.spect_evercddl_int_pretty_left_right
+                                COSE.Format.spect_evercddl_int_pretty_right_left
+                                (CDDL.Spec.EqTest.either_eq (CDDL.Pulse.Bundle.Base.mk_eq_test_bij COSE.Format.spect_evercddl_uint_pretty_right
+                                        COSE.Format.spect_evercddl_uint_pretty_left
+                                        COSE.Format.spect_evercddl_uint_pretty_left_right
+                                        COSE.Format.spect_evercddl_uint_pretty_right_left
+                                        (CDDL.Spec.EqTest.eqtype_eq FStar.UInt64.t))
+                                    (CDDL.Pulse.Bundle.Base.mk_eq_test_bij COSE.Format.spect_evercddl_nint_pretty_right
+                                        COSE.Format.spect_evercddl_nint_pretty_left
+                                        COSE.Format.spect_evercddl_nint_pretty_left_right
+                                        COSE.Format.spect_evercddl_nint_pretty_right_left
+                                        (CDDL.Spec.EqTest.eqtype_eq FStar.UInt64.t))))
+                            (CDDL.Pulse.Bundle.Base.mk_eq_test_bij COSE.Format.spect_evercddl_tstr_pretty_right
+                                COSE.Format.spect_evercddl_tstr_pretty_left
+                                COSE.Format.spect_evercddl_tstr_pretty_left_right
+                                COSE.Format.spect_evercddl_tstr_pretty_right_left
+                                (CDDL.Spec.EqTest.eqtype_eq (FStar.Seq.Base.seq FStar.UInt8.t))))))
+                COSE.Format.rel_aux_env25_type_2
+                COSE.Format.rel_aux_env25_type_4)
+
+let dummy_map_val () : aux_env25_type_2_pretty & aux_env25_type_4_pretty =
+  let zero: evercddl_int_pretty = Mkevercddl_int_pretty0 (Mkevercddl_uint_pretty0 0uL) in
+  Mkaux_env25_type_2_pretty0 (Mkevercddl_label_pretty0 zero),
+  Mkaux_env25_type_4_pretty0 (Mkevercddl_values_pretty0 (Mkevercddl_any_pretty0
+    { c = CBOR.Pulse.API.Det.Type.dummy_cbor_det_t (); p = 0.5R }))
+
+let assert_norm' (p: prop) : Pure (squash p) (requires normalize p) (ensures fun _ -> True) = ()
+
+let rel_inl_map_eq x y = assert_norm' (rel_inl_map x y == 
+  (exists* l . rel_slice_of_list (rel_pair rel_aux_env25_type_2 rel_aux_env25_type_4) false x l **
+      pure (y == map_of_list_pair ((CDDL.Pulse.Bundle.Base.mk_eq_test_bij
+                    COSE.Format.spect_aux_env25_type_2_pretty_right
+                    COSE.Format.spect_aux_env25_type_2_pretty_left
+                    COSE.Format.spect_aux_env25_type_2_pretty_left_right
+                    COSE.Format.spect_aux_env25_type_2_pretty_right_left
+                    (CDDL.Pulse.Bundle.Base.mk_eq_test_bij COSE.Format.spect_evercddl_label_pretty_right
+                        COSE.Format.spect_evercddl_label_pretty_left
+                        COSE.Format.spect_evercddl_label_pretty_left_right
+                        COSE.Format.spect_evercddl_label_pretty_right_left
+                        (CDDL.Spec.EqTest.either_eq (CDDL.Pulse.Bundle.Base.mk_eq_test_bij COSE.Format.spect_evercddl_int_pretty_right
+                                COSE.Format.spect_evercddl_int_pretty_left
+                                COSE.Format.spect_evercddl_int_pretty_left_right
+                                COSE.Format.spect_evercddl_int_pretty_right_left
+                                (CDDL.Spec.EqTest.either_eq (CDDL.Pulse.Bundle.Base.mk_eq_test_bij COSE.Format.spect_evercddl_uint_pretty_right
+                                        COSE.Format.spect_evercddl_uint_pretty_left
+                                        COSE.Format.spect_evercddl_uint_pretty_left_right
+                                        COSE.Format.spect_evercddl_uint_pretty_right_left
+                                        (CDDL.Spec.EqTest.eqtype_eq FStar.UInt64.t))
+                                    (CDDL.Pulse.Bundle.Base.mk_eq_test_bij COSE.Format.spect_evercddl_nint_pretty_right
+                                        COSE.Format.spect_evercddl_nint_pretty_left
+                                        COSE.Format.spect_evercddl_nint_pretty_left_right
+                                        COSE.Format.spect_evercddl_nint_pretty_right_left
+                                        (CDDL.Spec.EqTest.eqtype_eq FStar.UInt64.t))))
+                            (CDDL.Pulse.Bundle.Base.mk_eq_test_bij COSE.Format.spect_evercddl_tstr_pretty_right
+                                COSE.Format.spect_evercddl_tstr_pretty_left
+                                COSE.Format.spect_evercddl_tstr_pretty_left_right
+                                COSE.Format.spect_evercddl_tstr_pretty_right_left
+                                (CDDL.Spec.EqTest.eqtype_eq (FStar.Seq.Base.seq FStar.UInt8.t))))))
+      ) l)))
+
+module V = Pulse.Lib.Vec
+
+let sign1_phdrs_spec (alg: Int32.t) =
+  Mkspect_evercddl_empty_or_serialized_map_pretty0
+    (Mkspect_evercddl_header_map_pretty0
+      (Some (Inl (specint_of_i32 alg)))
+      None None None (Inr (Inr (None, None)))
+      (CDDL.Spec.Map.empty _ _))
+
+let rel_map_sign1_phdrs_eq (alg: Int32.t) alg' rest =
+  assert_norm' (rel_evercddl_empty_or_serialized_map (Mkevercddl_empty_or_serialized_map_pretty0
+    (Mkevercddl_header_map_pretty0 (Some (Inl alg')) None None None (Inr (Inr (None, None)))
+      (Inl { s = rest; p=1.0R })))
+    (sign1_phdrs_spec alg) ==
+    (((((rel_evercddl_int alg' (specint_of_i32 alg) **
+      emp) ** emp) ** emp) ** (emp ** emp)) **
+      rel_inl_map { s = rest; p=1.0R } (CDDL.Spec.Map.empty _ _)))
+
+fn mk_phdrs (alg: Int32.t)
+  returns res: evercddl_empty_or_serialized_map_pretty
+  ensures rel_evercddl_empty_or_serialized_map res (sign1_phdrs_spec alg)
+{
+  let alg' = mk_int alg;
+  let rest = V.alloc (dummy_map_val ()) 0sz;
+  V.to_array_pts_to rest;
+  let rest2 = S.from_array (V.vec_to_array rest) 0sz;
+  Pulse.Lib.SeqMatch.seq_list_match_nil_intro (Seq.Base.create 0 (dummy_map_val ())) []
+      (rel_pair rel_aux_env25_type_2 rel_aux_env25_type_4);
+  fold rel_slice_of_list (rel_pair rel_aux_env25_type_2 rel_aux_env25_type_4) false
+      (Mkslice rest2 1.0R) [];
+  rw_l (rel_inl_map_eq {s = rest2; p=1.0R} (CDDL.Spec.Map.empty _ _));
+  rw_l (rel_map_sign1_phdrs_eq alg alg' _);
+  with res. assert rel_evercddl_empty_or_serialized_map res (sign1_phdrs_spec alg);
+  drop_ (S.is_from_array (V.vec_to_array rest) rest2); // TODO leak
+
+  let alg'':
+        FStar.Tactics.PrettifyType.named "intkey1"
+              (FStar.Pervasives.either COSE.Format.evercddl_int_pretty
+                  COSE.Format.evercddl_tstr_pretty)
+  = Inl alg';
+  let foo:
+  FStar.Pervasives.either (FStar.Tactics.PrettifyType.named "intkey6"
+                  COSE.Format.evercddl_bstr_pretty &
+                FStar.Tactics.PrettifyType.named "intkey5"
+                  (FStar.Pervasives.Native.option (FStar.Tactics.PrettifyType.named "intkey5"
+                          COSE.Format.evercddl_everparsenomatch_pretty)))
+              (FStar.Tactics.PrettifyType.named "intkey6"
+                  (FStar.Pervasives.Native.option (FStar.Tactics.PrettifyType.named "intkey6"
+                          COSE.Format.evercddl_everparsenomatch_pretty)) &
+                FStar.Tactics.PrettifyType.named "intkey5"
+                  (FStar.Pervasives.Native.option (FStar.Tactics.PrettifyType.named "intkey5"
+                          COSE.Format.evercddl_everparsenomatch_pretty)))
+  = Inr (None, None);
+  let foo':
+        FStar.Pervasives.either (FStar.Tactics.PrettifyType.named "intkey5"
+              COSE.Format.evercddl_bstr_pretty &
+            FStar.Tactics.PrettifyType.named "intkey6"
+              (FStar.Pervasives.Native.option (FStar.Tactics.PrettifyType.named "intkey6"
+                      COSE.Format.evercddl_everparsenomatch_pretty)))
+          (FStar.Pervasives.either (FStar.Tactics.PrettifyType.named "intkey6"
+                  COSE.Format.evercddl_bstr_pretty &
+                FStar.Tactics.PrettifyType.named "intkey5"
+                  (FStar.Pervasives.Native.option (FStar.Tactics.PrettifyType.named "intkey5"
+                          COSE.Format.evercddl_everparsenomatch_pretty)))
+              (FStar.Tactics.PrettifyType.named "intkey6"
+                  (FStar.Pervasives.Native.option (FStar.Tactics.PrettifyType.named "intkey6"
+                          COSE.Format.evercddl_everparsenomatch_pretty)) &
+                FStar.Tactics.PrettifyType.named "intkey5"
+                  (FStar.Pervasives.Native.option (FStar.Tactics.PrettifyType.named "intkey5"
+                          COSE.Format.evercddl_everparsenomatch_pretty))))
+   = Inr foo;
+  let bar':
+        FStar.Pervasives.either (CDDL.Pulse.Types.slice (COSE.Format.aux_env25_type_2_pretty &
+                COSE.Format.aux_env25_type_4_pretty))
+          (CDDL.Pulse.Parse.MapGroup.map_iterator_t CBOR.Pulse.API.Det.Type.cbor_det_map_iterator_t
+              COSE.Format.aux_env25_type_2_pretty
+              COSE.Format.aux_env25_type_4_pretty
+              CBOR.Pulse.API.Det.C.cbor_det_match
+              (CDDL.Pulse.Iterator.Base.mk_spec COSE.Format.rel_aux_env25_type_2)
+              (CDDL.Pulse.Iterator.Base.mk_spec COSE.Format.rel_aux_env25_type_4))
+  = Inl { s = rest2; p=1.0R };
+  rewrite each res as Mkevercddl_empty_or_serialized_map_pretty0 (Mkevercddl_header_map_pretty0 (Some alg'') None None None foo' bar');
+  Mkevercddl_empty_or_serialized_map_pretty0 (Mkevercddl_header_map_pretty0 (Some alg'') None None None foo' bar')
+}
+
+let sign1_emphdrs_spec () : GTot _ =
+    (Mkspect_evercddl_header_map_pretty0
+      None None None None (Inr (Inr (None, None)))
+      (CDDL.Spec.Map.empty _ _))
+
+let rel_map_sign1_emphdrs_eq rest =
+  assert_norm' (rel_evercddl_header_map (
+    (Mkevercddl_header_map_pretty0 None None None None (Inr (Inr (None, None)))
+      (Inl { s = rest; p=1.0R })))
+    (sign1_emphdrs_spec ()) ==
+    (((((emp ** emp) ** emp) ** emp) ** (emp ** emp)) **
+      rel_inl_map { s = rest; p=1.0R } (CDDL.Spec.Map.empty _ _)))
+
+fn mk_emphdrs ()
+  returns res: evercddl_header_map_pretty
+  ensures rel_evercddl_header_map res (sign1_emphdrs_spec ())
+{
+  // let alg' = mk_int alg;
+  let rest = V.alloc (dummy_map_val ()) 0sz;
+  V.to_array_pts_to rest;
+  let rest2 = S.from_array (V.vec_to_array rest) 0sz;
+  Pulse.Lib.SeqMatch.seq_list_match_nil_intro (Seq.Base.create 0 (dummy_map_val ())) []
+      (rel_pair rel_aux_env25_type_2 rel_aux_env25_type_4);
+  fold rel_slice_of_list (rel_pair rel_aux_env25_type_2 rel_aux_env25_type_4) false
+      (Mkslice rest2 1.0R) [];
+  rw_l (rel_inl_map_eq {s = rest2; p=1.0R} (CDDL.Spec.Map.empty _ _));
+  rw_l (rel_map_sign1_emphdrs_eq _);
+  with res. assert rel_evercddl_header_map res (sign1_emphdrs_spec ());
+  drop_ (S.is_from_array (V.vec_to_array rest) rest2); // TODO leak
+  let foo:
+  FStar.Pervasives.either (FStar.Tactics.PrettifyType.named "intkey6"
+                  COSE.Format.evercddl_bstr_pretty &
+                FStar.Tactics.PrettifyType.named "intkey5"
+                  (FStar.Pervasives.Native.option (FStar.Tactics.PrettifyType.named "intkey5"
+                          COSE.Format.evercddl_everparsenomatch_pretty)))
+              (FStar.Tactics.PrettifyType.named "intkey6"
+                  (FStar.Pervasives.Native.option (FStar.Tactics.PrettifyType.named "intkey6"
+                          COSE.Format.evercddl_everparsenomatch_pretty)) &
+                FStar.Tactics.PrettifyType.named "intkey5"
+                  (FStar.Pervasives.Native.option (FStar.Tactics.PrettifyType.named "intkey5"
+                          COSE.Format.evercddl_everparsenomatch_pretty)))
+  = Inr (None, None);
+  let foo':
+        FStar.Pervasives.either (FStar.Tactics.PrettifyType.named "intkey5"
+              COSE.Format.evercddl_bstr_pretty &
+            FStar.Tactics.PrettifyType.named "intkey6"
+              (FStar.Pervasives.Native.option (FStar.Tactics.PrettifyType.named "intkey6"
+                      COSE.Format.evercddl_everparsenomatch_pretty)))
+          (FStar.Pervasives.either (FStar.Tactics.PrettifyType.named "intkey6"
+                  COSE.Format.evercddl_bstr_pretty &
+                FStar.Tactics.PrettifyType.named "intkey5"
+                  (FStar.Pervasives.Native.option (FStar.Tactics.PrettifyType.named "intkey5"
+                          COSE.Format.evercddl_everparsenomatch_pretty)))
+              (FStar.Tactics.PrettifyType.named "intkey6"
+                  (FStar.Pervasives.Native.option (FStar.Tactics.PrettifyType.named "intkey6"
+                          COSE.Format.evercddl_everparsenomatch_pretty)) &
+                FStar.Tactics.PrettifyType.named "intkey5"
+                  (FStar.Pervasives.Native.option (FStar.Tactics.PrettifyType.named "intkey5"
+                          COSE.Format.evercddl_everparsenomatch_pretty))))
+   = Inr foo;
+  let bar':
+        FStar.Pervasives.either (CDDL.Pulse.Types.slice (COSE.Format.aux_env25_type_2_pretty &
+                COSE.Format.aux_env25_type_4_pretty))
+          (CDDL.Pulse.Parse.MapGroup.map_iterator_t CBOR.Pulse.API.Det.Type.cbor_det_map_iterator_t
+              COSE.Format.aux_env25_type_2_pretty
+              COSE.Format.aux_env25_type_4_pretty
+              CBOR.Pulse.API.Det.C.cbor_det_match
+              (CDDL.Pulse.Iterator.Base.mk_spec COSE.Format.rel_aux_env25_type_2)
+              (CDDL.Pulse.Iterator.Base.mk_spec COSE.Format.rel_aux_env25_type_4))
+  = Inl { s = rest2; p=1.0R };
+  rewrite each res as (Mkevercddl_header_map_pretty0 None None None None foo' bar');
+  (Mkevercddl_header_map_pretty0 None None None None foo' bar')
+}
+
+let sign1_tagged_spec (alg: Int32.t) uhdr payload sig =
+  Mkspect_evercddl_COSE_Sign1_Tagged_pretty0 (Mkspect_evercddl_COSE_Sign1_pretty0
+    (sign1_phdrs_spec alg) uhdr (Inl payload) sig)
+
+// #push-options "--print_implicits"
+
+let rel_sign1_tagged_eq1 phdr uhdr payload sig vphdr vuhdr vpayload vsig =
+  assert_norm' (rel_evercddl_COSE_Sign1_Tagged
+      (Mkevercddl_COSE_Sign1_Tagged_pretty0
+        (Mkevercddl_COSE_Sign1_pretty0 phdr uhdr (Inl payload) sig))
+      (Mkspect_evercddl_COSE_Sign1_Tagged_pretty0 (Mkspect_evercddl_COSE_Sign1_pretty0
+        vphdr vuhdr (Inl vpayload) vsig)) ==
+  (rel_evercddl_empty_or_serialized_map phdr vphdr **
+    rel_evercddl_header_map uhdr vuhdr) **
+    (rel_evercddl_bstr payload vpayload ** rel_evercddl_bstr sig vsig))
+
+fn sign1 privkey uhdr aad payload (outbuf: S.slice UInt8.t)
+    #pprivkey (#vprivkey: erased (Seq.seq UInt8.t) { Seq.length vprivkey == 32 })
+    (#vuhdr: erased _) (#vaad: erased _) (#vpayload: erased _)
+    (#voutbuf: erased _)
+  requires AP.pts_to privkey #pprivkey vprivkey
+  requires rel_evercddl_header_map uhdr vuhdr
+  requires rel_evercddl_bstr aad vaad
+  requires rel_evercddl_bstr payload vpayload
+  requires pts_to outbuf voutbuf
+
+  returns outbuf_sz: SizeT.t
+  ensures AP.pts_to privkey #pprivkey vprivkey
+  // TODO leak leak
+  ensures rel_evercddl_header_map uhdr vuhdr
+  ensures rel_evercddl_bstr aad vaad
+  ensures rel_evercddl_bstr payload vpayload
+  ensures exists* voutbuf. pts_to outbuf voutbuf ** pure (SizeT.v outbuf_sz <= Seq.length voutbuf)
+  //  ** pure (SizeT.lt 0sz outbuf_sz ==> Seq.slice voutbuf 0 (SizeT.v outbuf_sz) == _)
+{
+  let alg: Int32.t = -8l;
+  let phdr = mk_phdrs alg;
+  let mut sigbuf = [| 0uy; 64sz |];
+  Seq.lemma_create_len (SizeT.v 64sz) 0uy; //?!?
+  let sigbuf2 = AP.from_array sigbuf;
+  create_sig privkey phdr aad payload sigbuf2;
+  AP.to_array sigbuf2 sigbuf #_ #(spec_ed25519_sign vprivkey _);
+  // let uhdr = mk_emphdrs ();
+  rw_l (rel_sign1_tagged_eq1 phdr _ payload _ (sign1_phdrs_spec alg) _ vpayload _);
+  let outbuf_sz = serialize_COSE_Sign1_Tagged' _ outbuf;
+  rw_r (rel_sign1_tagged_eq1 phdr _ payload _ (sign1_phdrs_spec alg) _ vpayload _);
+  drop_ (rel_evercddl_empty_or_serialized_map phdr _);
+  if (outbuf_sz = 0sz) { abort (); 0sz } else {
+    outbuf_sz;
+  }
+}
+
+let rel_bstr_eq (x: evercddl_bstr_pretty) (y: spect_evercddl_bstr_pretty) =
+  assert_norm' (rel_evercddl_bstr x y ==
+    (match x, y with
+    | Mkevercddl_bstr_pretty0 { s; p }, Mkspect_evercddl_bstr_pretty0 y ->
+      pts_to s #p y ** pure (false == false))
+    // pts_to x._x0.s #x._x0.p y._x0 ** pure (false == false)
+    )
+
+fn sign1_simple privkey payload (outbuf: S.slice UInt8.t)
+    #pprivkey (#vprivkey: erased (Seq.seq UInt8.t) { Seq.length vprivkey == 32 })
+    (#vpayload: erased _)
+    (#voutbuf: erased _)
+  requires AP.pts_to privkey #pprivkey vprivkey
+  requires rel_evercddl_bstr payload vpayload
+  requires pts_to outbuf voutbuf
+
+  returns outbuf_sz: SizeT.t
+  ensures AP.pts_to privkey #pprivkey vprivkey
+  // TODO leak leak
+  // ensures rel_evercddl_empty_or_serialized_map uhdr vuhdr
+  ensures rel_evercddl_bstr payload vpayload
+  ensures exists* voutbuf. S.pts_to outbuf voutbuf ** pure (SizeT.v outbuf_sz <= Seq.length voutbuf)
+  //  ** pure (SizeT.lt 0sz outbuf_sz ==> Seq.slice voutbuf 0 (SizeT.v outbuf_sz) == _)
+{
+  let uhdr = mk_emphdrs ();
+  let mut aadbuf = [| 0uy; 0sz |];
+  let aadslice = S.from_array aadbuf 0sz;
+  with aad. assert pure ((aad <: evercddl_bstr_pretty) == Mkevercddl_bstr_pretty0 { s = aadslice; p = 1.0R });
+  rw_l (rel_bstr_eq aad (Mkspect_evercddl_bstr_pretty0 _));
+  let res = sign1 privkey uhdr aad payload outbuf;
+  rw_r (rel_bstr_eq aad (Mkspect_evercddl_bstr_pretty0 _));
+  S.to_array aadslice;
+  drop_ (rel_evercddl_header_map uhdr _); // TODO leak
+  res
 }
 
 fn main () returns exitcode: Int32.t { 0l }
