src/cbor/pulse/CBOR.Pulse.API.Det.Type.fsti
@@ -9,5 +9,4 @@ val cbor_det_array_iterator_t: Type0
 [@@CAbstractStruct]
 val cbor_det_map_iterator_t: Type0
 
-inline_for_extraction noextract [@@noextract_to "krml"]
 val dummy_cbor_det_t (_: unit) : cbor_det_t
